theories/Real.ec
@@ -32,7 +32,9 @@ export FromInt.
 theory PowerInt.
   import why3 "real" "PowerInt"
      op "power" as "^".
-     
+  axiom pow_inv_pos :
+    forall (x : real) (n : int), Int.(<=) 0 n => x ^ (Int.([-]) n) = inv (x ^ n).
+   
 end PowerInt.
 export PowerInt.
 
@@ -60,5 +62,67 @@ lemma mulrM: forall (x y z:real),
   x * z < y * z
 by [].
 
+
 op exp : real -> real.
 (* TODO : add axioms*)
+
+require import AlgTactic.
+
+instance ring with real
+  op rzero = zero
+  op rone  = one
+  op add   = ( + )
+  op opp   = ([-])
+  op mul   = ( * )
+  op expr  = PowerInt.( ^ )
+  op sub   = (-)
+  op ofint = FromInt.from_int
+
+  proof oner_neq0 by smt
+  proof addr0     by smt
+  proof addrA     by smt
+  proof addrC     by smt
+  proof addrN     by smt
+  proof mulr1     by smt
+  proof mulrA     by smt
+  proof mulrC     by smt
+  proof mulrDl    by smt
+  proof expr0     by smt
+  proof exprS     by smt
+  proof subrE     by smt
+  proof ofint0    by smt
+  proof ofint1    by smt
+  proof ofintS    by smt
+  proof ofintN    by smt.
+
+instance field with real
+  op rzero = zero
+  op rone  = one
+  op add   = ( + )
+  op opp   = ([-])
+  op mul   = ( * )
+  op expr  = PowerInt.( ^ )
+  op sub   = (-)
+  op ofint = FromInt.from_int
+  op inv   = inv
+  op div   = (/)
+
+  proof oner_neq0 by smt
+  proof addr0     by smt
+  proof addrA     by smt
+  proof addrC     by smt
+  proof addrN     by smt
+  proof mulr1     by smt
+  proof mulrA     by smt
+  proof mulrC     by smt
+  proof mulrDl    by smt
+  proof mulrV     by smt
+  proof expr0     by smt
+  proof exprS     by smt
+  proof exprN     by smt
+  proof subrE     by smt
+  proof divrE     by smt
+  proof ofint0    by smt
+  proof ofint1    by smt
+  proof ofintS    by smt
+  proof ofintN    by smt.
